



# I Wedderburn-Artin Theory

## 1 Terminology and Examples

### Remark 1.19

$M$  noeth and artin iff  $M$  has a comp series.

### Proof.

Suppose  $M$  is both noetherian and artinian. Then,  $M$  has a maximal submodule  $N_1$ , by considering all proper submodules of  $M$  under inclusion. Similarly,  $N_1$  has such a maximal submodule  $N_2$ .

Indeed, for any  $k$ , let  $N_k$  be the maximal submodule of  $N_{k-1}$ . Since any submodule of  $M$  is noetherian, this is well-defined. Thus, we have a chain of submodules:

$$\cdots < N_3 < N_2 < N_1 < M$$

Since  $M$  is artinian, there is some  $k$  such that  $N_k = N_{k+1} = \dots$ . In other words, the chain terminates:

$$\{0\} = N_k < N_{k-1} < \cdots < N_2 < N_1 < M$$

Since each  $N_k$  is maximal in  $N_{k-1}$  by construction, then  $N_k/N_{k-1}$  is simple for all  $k$ . Thus,  $M$  has a composition series as needed. ■




**Remark 1.20**

$N$  submod of  $M$ . then  $M$  noeth iff  $N, M/N$  noeth

**Proof.**

First, notice that if  $N$  and  $A/N$  are f.g., then so is  $A$ . Indeed, suppose:

$$N = \langle x_1, \dots, x_n \rangle \quad A/N = \langle \bar{y}_1, \dots, \bar{y}_m \rangle$$

Let  $a \in A$ . Then:

$$\bar{a} = \sum_{i=1}^m s_i \bar{y}_i = \overline{\sum_{i=1}^m s_i y_i} \implies a - \sum_{i=1}^m s_i y_i = \sum_{j=1}^n r_j x_j$$

Thus, we have that  $A = \langle x_1, \dots, x_n, y_1, \dots, y_m \rangle$ .

Now, suppose  $N$  and  $M/N$  are noetherian. Let  $A \leq M$  be any submodule. By the Second Isomorphism Theorem, we have:

$$\frac{A}{A \cap N} \simeq \frac{A + N}{N} \leq \frac{M}{N}$$

Since  $A \cap N \leq N$  is f.g. and  $A/(A \cap N) \leq M/N$  is f.g., by the above, it follows that  $A$  is f.g., and thus  $M$  is noetherian.

Next, suppose  $M$  is noetherian. Then  $N$  is clearly noetherian, so let  $A$  be any submodule of  $M/N$ . By the Fourth(\*) Isomorphism Theorem,  $A \simeq L/N$  for some submodule  $N \leq L \leq M$ .

But since  $M$  noetherian,  $N$  and  $L$  are finitely generated, so it follows that  $A$  is finitely generated. ■




**Proposition 1.21(b)**

$R$  right noeth,  $M_R$  f.g.. then  $M_R$  noeth.

**Proof.**

Suppose  $M = \langle m_1, \dots, m_n \rangle$  for some  $n$ . Then:

$$m = \sum_{i=1}^n r_i m_i$$

for all  $m \in M$ .

Consider  $R^n = R \times R \times \dots \times R$ . We have a map  $\varphi : R^n \longrightarrow M$  given by:

$$\varphi(r_1, \dots, r_n) = \sum_{i=1}^n r_i m_i$$

Clearly,  $\varphi$  is surjective. Furthermore, since  $R$  is noetherian,  $R^n$  is as well. Therefore, by the First Isomorphism Theorem, we have that

$$\frac{R^n}{\ker(\varphi)} \simeq M$$

is noetherian as needed. ■

**Exercise 1.7a**

Source: Primary Source Material

Suppose  $R = I_1 \oplus \cdots \oplus I_n$  a direct sum of left ideals. show that  $I_k = Re_k$  for  $e_k$  idempotent elements of  $R$  satisfying  $e_1 + \cdots + e_n = 1$  and  $e_i e_j = 0$  for  $i \neq j$ .

**Proof.**

Since we can write  $R = I_1 \oplus \cdots \oplus I_n$ , then for all  $r \in R$ , there exists a unique linear combination such that:

$$r = \sum_{k=1}^n r_k \quad r_k \in I_k$$

In particular, there is a unique linear combination to write  $1 = e_1 + \cdots + e_n$ . Now, note that each  $r_k \in I_k$  can be written as:

$$r_k = \sum_{j=1}^n r_k \delta_{jk}$$

where  $\delta_{jk}$  is the Kronecker delta. In particular, this holds for each  $e_k$ ; it immediately follows that they are idempotent. We also see that for any  $r_k \in I_k$ :

$$r_k = r_k 1 = \left( \sum_{j=1}^n r_k \delta_{jk} \right) \left( \sum_{k=1}^n e_k \right) = \sum_{j=1}^n r_k \delta_{jk} e_k = r_k e_k$$

So  $I_k = Re_k$  as needed. Finally, we have that  $e_j e_k = 0$  for  $j \neq k$ , since:

$$e_j e_k = \left( \sum_{i=1}^n e_j \delta_{ij} \right) \left( \sum_{i=1}^n e_k \delta_{ik} \right) = \sum_{i=1}^n e_j \delta_{ij} e_k \delta_{ik} = 0$$

since  $j \neq k$ . ■



**Exercise 1.7b**

Source: Primary Source Material

show  $I_k$  is a ring w identity  $e_k$ , and  $R \simeq I_1 \times \cdots \times I_n$ .

**Proof.**

From part a), we saw that  $r_k = r_k e_k$  for all  $r_k \in I_k$ . The proof that  $r_k = e_k r_k$  is symmetric, so it remains to show that  $R \simeq I_1 \times \cdots \times I_n$ .

Indeed, suppose  $S$  is any ring with  $\varphi_k : S \longrightarrow I_k$  ring homomorphisms. Define:

$$\varphi : S \longrightarrow I_1 \oplus \cdots \oplus I_n \quad \varphi(s) := \varphi_1(s) + \cdots + \varphi_n(s)$$

We have  $\varphi(1) = 1$  since necessarily  $\varphi_k(1) = e_k$ ; clearly  $\varphi(a+b) = \varphi(a) + \varphi(b)$ . Now:

$$\varphi_i(a)\varphi_j(b) = \left( \sum_{k=1}^n \varphi_i(a)\delta_{ik} \right) \left( \sum_{k=1}^n \varphi_j(b)\delta_{jk} \right) = \varphi_i(a)\varphi_j(b)\delta_{ij}$$

where the Kronecker delta commutes, since it is either 0 or 1. This implies:

$$\begin{aligned} \varphi(ab) &= \sum_{k=1}^n \varphi_k(ab) = \sum_{k=1}^n \varphi_k(a)\varphi_k(b) = \sum_{i=1}^n \sum_{j=1}^n \varphi_i(a)\varphi_j(b) \\ &= \left( \sum_{i=1}^n \varphi_i(a) \right) \left( \sum_{j=1}^n \varphi_j(b) \right) \\ &= \varphi(a)\varphi(b) \end{aligned}$$

Therefore,  $\varphi$  is indeed a ring homomorphism. Define  $\pi_k : I_1 \oplus \cdots \oplus I_n \longrightarrow I_k$  as  $\pi_k(r) = r_k$ , where  $r = \sum_{k=1}^n r_k$ . This is well-defined by the uniqueness of the decomposition of  $r$ , and is clearly a ring homomorphism.

Finally, notice  $\varphi_k = \pi_k \circ \varphi$  for all  $k$ . Thus, by the universal property of products in the category **Ring**, we are done. ■



**Exercise 1.7c**

Source: Primary Source Material

show if  $I_k$  are two-sided ideals, then  $e_k \in Z(R)$ .

**Proof.**

First, recall that if  $j \neq k$ , then  $I_j \cap I_k = \{0\}$  must be trivial by uniqueness of decomposition. Then, it simply suffices to note that for any  $r \in R$ :

$$re_k = r_ke_k = r_k = e_kr_k = e_kr$$

by the above fact and work shown in previous parts. ■

**Exercise 1.8**

Source: Primary Source Material

Suppose  $R = I \oplus J$  for ideals  $I, J$ . show every ideal of  $R$  is of the form  $I' \oplus J'$ , where  $I', J'$  ideals in  $I, J$  resp.

**Proof.**

Suppose  $S \subseteq R$  is an ideal. By Exercise 1.7, there exists  $e_i \in I$  and  $e_j \in J$  such that  $I = Re_i, J = Re_j, e_i + e_j = 1$ , and  $e_i, e_j$  is the identity of  $I, J$  resp. as a ring. Define  $I' := Se_i$  and  $J' := Se_j$ . We want to show that  $S = I' \oplus J'$ .

Clearly  $I', J' \subseteq S$  since  $S$  is an ideal, thus  $I' + J' \subseteq S$ . On the other hand, for any  $s \in S$ , let:

$$s_i \in I', s_j \in J' \quad s_i := se_i \quad s_j := se_j$$

Then  $s_i + s_j = se_i + se_j = s(e_i + e_j) = s$ , so we see that  $S = I' + J'$ . Finally, since  $s_i \in I$  and  $s_j \in J$ , then  $s = s_i + s_j$  is the unique decomposition of  $s$ , and it follows that  $S = I' \oplus J'$  as needed. ■

**Exercise 1.12a**

Source: Primary Source Material

${}_R M$  is called *Hopfian* if every surj endo is inj. show every noeth  ${}_R M$  is hopfian.

**Proof.**

Let  $\varphi$  be a surjective endomorphism of  $M$ . Recall that  $\ker(\varphi)$  is a submodule of  $M$ . Consider  $\varphi^{(2)} := \varphi \circ \varphi$ . Since  $\varphi$  is surjective, then there exists  $m \in M$  such that  $\varphi(m) \in \ker(\varphi)$ . Thus, we have that  $\ker(\varphi) \leq \ker(\varphi^{(2)})$ .

In general, we can consider  $\ker(\varphi^{(k)})$  in the same way. Since  $\varphi$  is surjective, we have that  $\text{im}(\varphi^{(k)}) = M$ , so we can construct the following chain:

$$\ker(\varphi) \leq \ker(\varphi^{(2)}) \leq \ker(\varphi^{(3)}) \leq \dots$$

Since  $M$  is noetherian, this chain must terminate; if  $\ker(\varphi)$  is non-trivial, then the above construction holds. Therefore  $\ker(\varphi) = \{0\}$ , or in other words,  $\varphi$  is injective. ■

**Exercise 1.12b**

Source: Primary Source Material

prove  ${}_R R$  is hopfian iff dedekind-finite

**Proof.**

Source: Primary Source Material

First, suppose  ${}_R R$  is Hopfian and fix  $x \in R$  such that  $xy = 1$  for some  $y \in R$ . It suffices to show that  $x$  is left-invertible.

For any  $r \in R$ , let  $\varphi_r(s) = rs$ . This is evidently an endomorphism. Consider the map  $\varphi_x$ ; note that this is surjective, as it has a right-inverse:

$$(\varphi_x \circ \varphi_y)(s) = (xy)s = s \implies \varphi_x \circ \varphi_y = \varphi_1 = \text{id}$$

Since  $R$  is Hopfian, then  $\varphi_x$  is injective. By uniqueness of inverses, we have:

$$(\varphi_y \circ \varphi_x)(s) = (yx)s = s$$







Since this is true of all  $s \in R$ , then  $yx = 1$  as needed.

Now, suppose  $R$  is Dedekind-finite. Let  $\varphi : R \longrightarrow R$  be a surjective endomorphism. Notice:

$$\varphi(r) = \varphi(1r) = \varphi(1)r$$

Thus  $\varphi = \varphi_{\varphi(1)}$  is given by scaling. Fix  $\varphi(1) = r$ . Since  $\varphi$  is surjective, then there exists some  $s \in R$  such that:

$$\varphi(s) = rs = 1$$

Similarly to above, we therefore have that:

$$\varphi \circ \varphi_s = \varphi_r \circ \varphi_s = \varphi_1 = \text{id}$$

Since  $R$  is Dedekind-finite, then:

$$\varphi_s \circ \varphi = \varphi_s \circ \varphi_r = \varphi_1 = \text{id}$$

It follows that  $\varphi$  is injective, and so  $R$  is indeed Hopfian. ■

**Exercise 1.13a**

Source: Primary Source Material

Show that if  $R$  is finite-dimensional as a  $k$ -vector space,  $R$  is algebraic. Is the converse true?

**Proof.**

Suppose  $R$  is finite-dimensional as a  $k$ -vector space, and fix  $r \in R$ . Let  $s \in R$  be any element, and consider the endomorphism  $\varphi_r$  given as  $\varphi_r(s) = rs$ .

Since  $R$  is a  $k$ -algebra and  $\varphi_r$  is an endomorphism, we must have that  $\varphi_r$  is given by some square matrix  $A$ . Let  $p \in k[x]$  be the characteristic polynomial of  $A$ . We claim that  $p(r) = 0$ .

Write the characteristic polynomial  $p(x)$  of  $A$  as:

$$p(x) := a_n x^n + \cdots + a_1 x + a_0$$

where each  $a_i \in k$ . Then:

$$\begin{aligned} p(r) &= p(r) \cdot 1 = (a_n r^n + \cdots + a_1 r + a_0) \cdot 1 = a_n r^n \cdot 1 + \cdots + a_1 r \cdot 1 + a_0 \cdot 1 \\ &= a_n A^n \cdot 1 + \cdots + a_1 A \cdot 1 + a_0 I_n \cdot 1 \\ &= a_n A^n + \cdots + a_1 A + a_0 I_n \\ &= 0 \end{aligned}$$

by the Cayley-Hamilton theorem. Therefore we have that  $p(r) = 0$  as needed.

NOTE: idk for converse



**Exercise 1.13b**

Source: Primary Source Material

Henceforth, let  $R$  be an algebraic  $k$ -algebra. Show  $R$  is Dedekind-finite.

**Proof.**

Suppose  $r, s \in R$  such that  $rs = 1$ . Since  $R$  is algebraic, there exists  $p \in k[x]$  such that  $p(r) = 0$ . Write:

$$p(x) := a_n x^n + \cdots + a_1 x + a_0$$

Suppose  $m$  is the lowest index such that  $a_m \neq 0$ . Then:

$$p(r) \cdot s^m = (a_n r^n + \cdots + a_m r^m) s^m = a_n r^{n-m} + \cdots + a_{m+1} r + a_m = 0$$

Thus, suppose WLOG that  $a_0 \neq 0$ . Then:

$$\begin{aligned} a_n r^n + \cdots + a_1 r + a_0 = 0 &\implies a_n r^n + \cdots + a_1 r = -a_0 \\ &\implies (a_n r^{n-1} + \cdots + a_2 r + a_1) r = -a_0 \\ &\implies -(a_0^{-1}) (a_n r^{n-1} + \cdots + a_2 r + a_1) r = 1 \end{aligned}$$

since  $a_0 \in k$ , and  $k$  is a field. Thus,  $r$  has a left-inverse, so by uniqueness of inverses, we have  $sr = 1$ . ■

**Exercise 1.13c**

Source: Primary Source Material

Show that every left zero divisor is also a right zero divisor.

**Proof.**

incomplete ■

**Exercise 1.13d**

Source: Primary Source Material

Suppose  $r \in R$  is non-zero. Show that  $r$  is a zero divisor iff it is not a unit.

**Proof.**

If  $r$  is a unit, then  $r$  cannot be a (left) zero divisor as:

$$rs = 0 \implies s = r^{-1}rs = r^{-1} \cdot 0 = 0 \quad sr = 0 \implies s = srr^{-1} = 0 \cdot r^{-1} = 0$$

On the other hand, if  $r$  is not a (left) zero divisor, then the map  $\varphi_r(s) = rs$  is injective. Thus, it has a (left-)inverse  $\varphi$ . Since  $\varphi$  is necessarily surjective,  $\varphi = \varphi_a$  for some  $a \in R$ . Then:

$$(\varphi_a \circ \varphi_r)(s) = ars = s \implies ar = 1$$

So  $r$  has a (left-)inverse.

Since the sided-ness does not affect either argument, we are done. ■

**Exercise 1.13e**

Source: Primary Source Material

Let  $B$  be a  $k$ -subalgebra of  $R$ ,  $b \in B$ . Show that if  $b$  is a unit in  $R$ , then  $b^{-1} \in B$ .

**Proof.**

Since  $R$  is algebraic, there exists non-zero  $p \in k[x]$  such that  $p(b) = 0$ . Note that:

$$p(b) = a_nb^n + \cdots + a_1b + a_0 = 0 \implies b \cdot \left( \frac{-1}{a_0}(a_nb^{n-1} + \cdots + a_2b + a_1) \right) = b \cdot b^{-1} = 1$$

by the same argument as in part b). By uniqueness of inverses,  $b^{-1} \in B$  as needed.

NOTE: a little unsure about this one ■

